src/Ast/Resolver.dfy
@@ -16,15 +16,15 @@ module Resolver {
     var intType := new Type(IntTypeName);
     var typeMap := map[BoolTypeName := boolType, IntTypeName := intType];
     for n := 0 to |b3.types|
-      // invariants about typeMap
+      // typeMap maps built-in types and the user-defined types seen so far to distinct type-declaration objects
       invariant typeMap.Keys == BuiltInTypes + set typename <- b3.types[..n]
       invariant MapIsInjective(typeMap)
-      // invariants related to showing we've checked the conditions of RawAst well-formedness
-      invariant forall typename <- b3.types[..n] :: typename !in BuiltInTypes
-      invariant forall i, j :: 0 <= i < j < n ==> b3.types[i] != b3.types[j]
-      // invariants related to showing that the resolved declarations are well-formed
-      invariant BuiltInTypes <= (set typ: Type <- typeMap.Values :: typ.Name)
+      // typeMap organizes type-declaration objects correctly according to their names
       invariant forall typename <- typeMap.Keys :: typeMap[typename].Name == typename
+      // no user-defined type seen so far uses the name of a built-in type
+      invariant forall typename <- b3.types[..n] :: typename !in BuiltInTypes
+      // the user-defined types seen so far have distinct names
+      invariant forall i, j :: 0 <= i < j < n ==> b3.types[i] != b3.types[j]
     {
       var name := b3.types[n];
       if name in typeMap.Keys {
@@ -36,14 +36,15 @@ module Resolver {
 
     var procMap: map<string, Procedure> := map[];
     for n := 0 to |b3.procedures|
-      // invariants about procMap
+      // procMap maps the user-defined procedures seen so far to distinct procedure-declaration objects
       invariant procMap.Keys == set proc <- b3.procedures[..n] :: proc.name
       invariant MapIsInjective(procMap)
-      // invariants related to showing we've checked the conditions of RawAst well-formedness
-      invariant forall i, j :: 0 <= i < j < n ==> b3.procedures[i].name != b3.procedures[j].name
-      invariant forall proc <- b3.procedures[..n] :: proc.WellFormed(b3)
-      // invariants related to showing that the resolved declarations are well-formed
+      // procMap organizes procedure-declaration objects correctly according to their names
       invariant forall procname <- procMap.Keys :: procMap[procname].Name == procname
+      // user-defined types seen so far have distinct names
+      invariant forall i, j :: 0 <= i < j < n ==> b3.procedures[i].name != b3.procedures[j].name
+      // the procedures seen so far are well-formed
+      invariant forall proc <- b3.procedures[..n] :: proc.WellFormed(b3)
     {
       var proc := b3.procedures[n];
       var name := proc.name;
@@ -63,12 +64,22 @@ module Resolver {
     ensures r.Success? ==> proc.WellFormed(b3)
     ensures r.Success? ==> r.value.Name == proc.name
   {
-    if i, j :| 0 <= i < j < |proc.parameters| && proc.parameters[i].v.name == proc.parameters[j].v.name {
-      return Failure("duplicate parameter name: " + proc.parameters[i].v.name);
+    if i, j :| 0 <= i < j < |proc.parameters| && proc.parameters[i].name == proc.parameters[j].name {
+      return Failure("duplicate parameter name: " + proc.parameters[i].name);
     }
-    assert Raw.Variable.UniqueNames(SeqMap(proc.parameters, (p: Parameter) => p.v));
 
-    var rproc := new Procedure(proc.name, [], Nil, Nil); // TODO: other parameters
+/*
+    // TODO: remove 
+      && var preScope := map p <- parameters | p.kind.IsIncomingParameter() :: p.name := p;
+      && pre.Forall((ae: AExpr) requires ae < this => ae.WellFormed(b3, preScope, {}))
+      && var scope := map p <- parameters :: p.name := p;
+      && post.Forall((ae: AExpr) requires ae < this => ae.WellFormed(b3, scope, {}))
+      && var localNames := set p <- parameters | p.kind.IsOutgoingParameter() :: p.name;
+      && (body == None || body.value.WellFormed(b3, scope, localNames, {}))
+*/
+
+
+    var rproc := new Procedure(proc.name, [], [], []); // TODO: other parameters
     assume {:axiom} proc.WellFormed(b3); // TODO
     return Success(rproc);
   }
